making instatiations of equations work, both on representations and on high-level effectful code

Eff.Template.Equation.Test.fst
@@ -16,92 +16,62 @@ let rw : sig = r `union` w
 
 (* State equations using templates *)
 
-let st_eq1 a : equation a rw 
+let st_eq1 : equation rw 
   = { 
       vctx = [];
       cctx = [unit];
-      lhs  = (fun vvars cvars -> let y = perform read () in 
-                              let y' = perform write y in
-                              cvar cvars 0 y');
-      rhs  = (fun vvars cvars -> cvar cvars 0 ())
+      lhs  = (fun vvars -> let y = perform read () in 
+                        let y' = perform write y in
+                        cvar 0 y');
+      rhs  = (fun vvars -> cvar 0 ())
     }
 
-let st_eq2 a : equation a rw
+let st_eq2 : equation rw
   = {
       vctx = [int];
       cctx = [int];
-      lhs  = (fun vvars cvars -> perform write (vvar vvars 0);
-                              let y = perform read () in
-                              cvar cvars 0 y);
-      rhs  = (fun vvars cvars -> perform write (vvar vvars 0);
-                              cvar cvars 0 (vvar vvars 0))
+      lhs  = (fun vvars -> perform write (vvar vvars 0);
+                        let y = perform read () in
+                        cvar 0 y);
+      rhs  = (fun vvars -> perform write (vvar vvars 0);
+                        cvar 0 (vvar vvars 0))
     }
 
-let st_eq3 a : equation a rw
+let st_eq3 : equation rw
   = {
       vctx = [int;int];
       cctx = [unit];
-      lhs  = (fun vvars cvars -> perform write (vvar vvars 0);
-                              let y = perform write (vvar vvars 1) in
-                              cvar cvars 0 y);
-      rhs  = (fun vvars cvars -> let y = perform write (vvar vvars 1) in
-                              cvar cvars 0 y)
+      lhs  = (fun vvars -> perform write (vvar vvars 0);
+                        let y = perform write (vvar vvars 1) in
+                        cvar 0 y);
+      rhs  = (fun vvars -> let y = perform write (vvar vvars 1) in
+                        cvar 0 y)
     }
 
 
 
 
 
+(* ************************** *)
 
 
-
-(*
-
-(* ********************** *)
-(* ********************** *)
-(* ********************** *)
-
-
-open FStar.Tactics
-
-let foo a ops (z:int -> template_repr a ops)
-  : Lemma (to_cvars #[int] [RCVar int z] == [CVar int (reflect_cont #a #int #ops z)])
-  = ()
-
-(*
-let foobar a ops (z1:int -> Template a ops) (z2:int -> template_repr a ops)
-  : Lemma (reify (perform read () z) == )
-  = ()
-*)
-
-let st_eq a : equation a rw
+let st_eq : equation rw
   = {
       vctx = [int;int;int];
       cctx = [unit];
-      lhs  = (fun vvars cvars -> perform write (vvar vvars 0);
-                              perform write (vvar vvars 1);
-                              let y = perform write (vvar vvars 2) in
-                              cvar cvars 0 y);
-      rhs  = (fun vvars cvars -> perform write (vvar vvars 0);
-                              let y = perform write (vvar vvars 2) in
-                              cvar cvars 0 y)
+      lhs  = (fun vvars -> perform write (vvar vvars 0);
+                        perform write (vvar vvars 1);
+                        let y = perform write (vvar vvars 2) in
+                        cvar 0 y);
+      rhs  = (fun vvars -> perform write (vvar vvars 0);
+                        let y = perform write (vvar vvars 2) in
+                        cvar 0 y)
     }
 
-let prop_st_eq3 a 
-  : prop
-  = repr_eq_to_prop (to_repr_eq (st_eq3 a))
 
-let prop_st_eq a 
-  : prop
-  = repr_eq_to_prop (to_repr_eq (st_eq a))
+assume val t : Type
 
-(*
-let bar a 
-  : Lemma (to_repr_eq (st_eq3 a) == to_repr_eq (st_eq a)) by (norm [delta; nbe]; dump "bar")
+let foo ()
+  : Lemma (requires (norm [delta;zeta;primops;simplify;iota] (eq_to_prop (to_inst_equation (to_template_equation st_eq3) (id_template_handler t rw)))))
+          (ensures  (norm [delta;zeta;primops;simplify;iota] (eq_to_prop (to_inst_equation (to_template_equation st_eq) (id_template_handler t rw)))))
   = ()
-
-let bar a : Lemma (requires (prop_st_eq3 a))
-                  (ensures  (prop_st_eq a)) by (norm [delta; nbe]; dump "foo")
-  = ()
-*)
-*)
