Eff.Template.Equation.fst
@@ -10,12 +10,14 @@ module L = FStar.List.Tot
 (* Equations between templates *)
 (* *************************** *)
 
-(* Value variables *)
+(* Value contexts and value variables *)
+
+let vctx = list Type0
 
 noeq type vvar_t =
-  | VVar : (a:Type) -> (x:a) -> vvar_t
+  | VVar : (a:Type0) -> (x:a) -> vvar_t
 
-let vvars_pred (vctx:list Type) (vvars:list vvar_t)
+let vvars_pred (vctx:vctx) (vvars:list vvar_t)
   = L.length vctx = L.length vvars /\
     (forall x . x < L.length vvars ==> VVar?.a (L.index vvars x) == (L.index vctx x))
 
@@ -27,104 +29,112 @@ let vvar #vctx (vvars:vvars vctx) (x:nat{x < L.length vctx})
   = VVar?.x (L.index vvars x)
 
 
-(* Computation variables *)
+(* Compuation contexts and compuation variables *)
 
-noeq type cvar_t a ops =
-  | CVar : (b:Type) -> (z:(b -> Template a ops)) -> cvar_t a ops
+let cctx = list Type0
 
-let cvars_pred (cctx:list Type) a ops (cvars:list (cvar_t a ops))
+noeq type cvar_t (cctx:cctx) =
+  | CVar : (x:nat{x < L.length cctx}) -> L.index cctx x -> cvar_t cctx
+
+let cvar (#cctx:cctx) (x:nat{x < L.length cctx}) (t:L.index cctx x) 
+  : cvar_t cctx
+  = CVar x t
+
+
+(* Equations between (direct-style, effectful) templates *)
+
+noeq type equation (ops:sig) = {
+  vctx:vctx;
+  cctx:cctx;
+  lhs:(vvars vctx) -> Template (cvar_t cctx) ops;
+  rhs:(vvars vctx) -> Template (cvar_t cctx) ops
+}
+
+
+(* Equations between (representations of) templates *)
+
+noeq type template_equation (ops:sig) = {
+  tvctx:vctx;
+  tcctx:cctx;
+  tlhs:(vvars tvctx) -> template (cvar_t tcctx) ops;
+  trhs:(vvars tvctx) -> template (cvar_t tcctx) ops
+}
+
+
+(* Translate a direct-style, effectful equation to a representation equation *)
+
+let to_template_equation #ops (eq:equation ops)
+  : template_equation ops
+  = {
+      tvctx = eq.vctx;
+      tcctx = eq.cctx;
+      tlhs  = (fun vvars -> reify (eq.lhs vvars));
+      trhs  = (fun vvars -> reify (eq.rhs vvars));
+    }
+
+
+(* Intatiated template equations *)
+
+noeq type inst_cvar_t a ops =
+  | ICVar : (b:Type0) -> (z:(b -> template a ops)) -> inst_cvar_t a ops
+
+let inst_cvars_pred (cctx:cctx) a ops (cvars:list (inst_cvar_t a ops))
   = L.length cctx = L.length cvars /\
-    (forall x . x < L.length cvars ==> CVar?.b (L.index cvars x) == (L.index cctx x))
+    (forall x . x < L.length cvars ==> ICVar?.b (L.index cvars x) == (L.index cctx x))
 
-let cvars cctx a ops
-  = cvars:list (cvar_t a ops){cvars_pred cctx a ops cvars}
-                             
-let cvar #cctx #a #ops (cvars:cvars cctx a ops) (x:nat{x < L.length cctx}) 
-  : (L.index cctx x) -> Template a ops
-  = CVar?.z (L.index cvars x)
+let inst_cvars cctx a ops
+  = cvars:list (inst_cvar_t a ops){inst_cvars_pred cctx a ops cvars}
 
-
-(* Equations between templates *)
-
-noeq type equation (a:Type) (ops:sig) = {
-  vctx:list Type;
-  cctx:list Type;
-  lhs:(vvars vctx) -> (cvars cctx a ops) -> Template a ops;
-  rhs:(vvars vctx) -> (cvars cctx a ops) -> Template a ops
+noeq type inst_equation (a:Type) (ops:sig) = {
+  ivctx:vctx;
+  icctx:cctx;
+  ilhs:(vvars ivctx) -> (inst_cvars icctx a ops) -> template a ops;
+  irhs:(vvars ivctx) -> (inst_cvars icctx a ops) -> template a ops
 }
 
 
+(* Intatiating a template equation (lhs/rhs) with a handler *)
 
-(* ********************************************************** *)
-(* Turning equations between templates into logical equations *)
-(* ********************************************************** *)
+let rec to_inst_template #a #ops #ops' #cctx
+  (t:template (cvar_t cctx) ops)
+  (h:template_handler ops a ops')
+  (cvars:inst_cvars cctx a ops')
+  : template a ops'
+  = match t with
+    | Leaf (CVar x u) ->
+        ICVar?.z (L.index cvars x) u
+    | Node op x k -> 
+        h op x (fun y -> to_inst_template (k y) h cvars)
 
-(* Computation variables for template representations *)
-
-noeq type repr_cvar_t a ops =
-  | RCVar : (b:Type) -> (z:(b -> template_repr a ops)) -> repr_cvar_t a ops
-
-let repr_cvars_pred (cctx:list Type) a ops (rcvars:list (repr_cvar_t a ops))
-  = L.length cctx = L.length rcvars /\
-    (forall x . x < L.length rcvars ==> RCVar?.b (L.index rcvars x) == (L.index cctx x))
-
-let repr_cvars (cctx:list Type) a ops
-  = rcvars:list (repr_cvar_t a ops){repr_cvars_pred cctx a ops rcvars}
-
-let repr_cvar #cctx #a #ops (rcvars:repr_cvars cctx a ops) (x:nat{x < L.length cctx}) 
-  : (L.index cctx x) -> template_repr a ops
-  = RCVar?.z (L.index rcvars x)
-
-
-(* Equations between the representations of templates *)
-
-noeq type repr_equation (a:Type) (ops:sig) = {
-  repr_vctx:list Type;
-  repr_cctx:list Type;
-  repr_lhs:(vvars repr_vctx) -> (repr_cvars repr_cctx a ops) -> template_repr a ops;
-  repr_rhs:(vvars repr_vctx) -> (repr_cvars repr_cctx a ops) -> template_repr a ops
-}
-
-let lemma_to_cvars_cons (cctx:list Type) a ops 
-                        (b:Type) (z:(b -> template_repr a ops))
-                        (rcvars:list (repr_cvar_t a ops))
-  : Lemma (requires (repr_cvars_pred (b :: cctx) a ops (RCVar b z :: rcvars)))
-          (ensures  (repr_cvars_pred cctx a ops rcvars))
-          [SMTPat (repr_cvars_pred (b :: cctx) a ops (RCVar b z :: rcvars))]
-  = assert (forall x . x < L.length rcvars ==> L.index rcvars x == L.index (RCVar b z :: rcvars) (x + 1))
-
-let rec to_cvars (#cctx:list Type) #a #ops (rcvars:repr_cvars cctx a ops)
-  : cvars cctx a ops 
-  = match rcvars with
-    | [] -> []
-    | (RCVar b z) :: rcvars -> 
-        match cctx with
-        | b' :: cctx -> (CVar b (reflect_cont #a #b #ops z)) :: to_cvars #cctx #a #ops rcvars
-
-let to_repr_eq #a #ops (eq:equation a ops) : repr_equation a ops = {
-    repr_vctx = eq.vctx;
-    repr_cctx = eq.cctx;
-    repr_lhs  = (fun vvars rcvars -> reify (eq.lhs vvars (to_cvars rcvars)));
-    repr_rhs  = (fun vvars rcvars -> reify (eq.rhs vvars (to_cvars rcvars)))
-}
+let to_inst_equation #a #ops #ops'
+  (eq:template_equation ops)
+  (h:template_handler ops a ops')
+  : inst_equation a ops' 
+  = {
+      ivctx = eq.tvctx;
+      icctx = eq.tcctx;
+      ilhs  = (fun vvars -> to_inst_template (eq.tlhs vvars) h);
+      irhs  = (fun vvars -> to_inst_template (eq.trhs vvars) h)
+    }
 
 
-(* Turning an equation on template representations into to a logical formula *)
+(* Turning an (instantiated) template equation into to a logical formula *)
 
-let rec repr_eq_to_prop #a #ops (eq:repr_equation a ops) 
-  : Tot prop (decreases %[eq.repr_vctx; eq.repr_cctx])
-  = match eq.repr_vctx with
-    | [] -> (match eq.repr_cctx with
-            | [] -> eq.repr_lhs [] [] `equiv` eq.repr_rhs [] []
+let rec eq_to_prop #a #ops (eq:inst_equation a ops) 
+  : Tot prop (decreases %[eq.ivctx; eq.icctx])
+  = match eq.ivctx with
+    | [] -> (match eq.icctx with
+            | [] -> eq.ilhs [] [] `equiv` eq.irhs [] []
             | b :: cctx -> 
-                forall (z:b -> template_repr a ops) . 
-                    repr_eq_to_prop ({ repr_vctx = eq.repr_vctx; 
-                                       repr_cctx = cctx;
-                                       repr_lhs  = (fun vvars rcvars -> eq.repr_lhs vvars (RCVar b z :: rcvars));
-                                       repr_rhs  = (fun vvars rcvars -> eq.repr_rhs vvars (RCVar b z :: rcvars)) }))
+                forall (z:b -> template a ops) . 
+                    eq_to_prop ({ ivctx = eq.ivctx; 
+                                  icctx = cctx;
+                                  ilhs  = (fun vvars rcvars -> eq.ilhs vvars (ICVar b z :: rcvars));
+                                  irhs  = (fun vvars rcvars -> eq.irhs vvars (ICVar b z :: rcvars)) }))
     | b :: vctx -> 
         forall (x:b) . 
-            repr_eq_to_prop ({ repr_vctx = vctx; 
-                               repr_cctx = eq.repr_cctx;
-                               repr_lhs  = (fun vvars rcvars -> eq.repr_lhs (VVar b x :: vvars) rcvars);
-                               repr_rhs  = (fun vvars rcvars -> eq.repr_rhs (VVar b x :: vvars) rcvars) })
+            eq_to_prop ({ ivctx = vctx; 
+                          icctx = eq.icctx;
+                          ilhs  = (fun vvars rcvars -> eq.ilhs (VVar b x :: vvars) rcvars);
+                          irhs  = (fun vvars rcvars -> eq.irhs (VVar b x :: vvars) rcvars) })
+
