Eff.Template.Equiv.fsti
@@ -3,18 +3,18 @@ module Eff.Template.Equiv
 open Eff.Signature
 open Eff.Template
 
-val equiv (#a:Type) (#ops:sig) (t1 t2:template_repr a ops) : prop
+val equiv (#a:Type) (#ops:sig) (t1 t2:template a ops) : prop
 
-val refl (#a:Type) (#ops:sig) (t:template_repr a ops)
+val refl (#a:Type) (#ops:sig) (t:template a ops)
   : Lemma (t `equiv` t)
           [SMTPat (t `equiv` t)]
 
-val sym (#a:Type) (#ops:sig) (t1 t2:template_repr a ops)
+val sym (#a:Type) (#ops:sig) (t1 t2:template a ops)
   : Lemma (requires (t1 `equiv` t2))
           (ensures  (t2 `equiv` t1))
           [SMTPat (t2 `equiv` t1)]
 
-val trans (#a:Type) (#ops:sig) (t1 t2 t3:template_repr a ops)
+val trans (#a:Type) (#ops:sig) (t1 t2 t3:template a ops)
   : Lemma (requires (t1 `equiv` t2 /\ t2 `equiv` t3))
           (ensures  (t1 `equiv` t3))
           [SMTPat (t1 `equiv` t2); 
@@ -27,7 +27,7 @@ val leaf_cong (#a:Type) (#ops:sig) (x1 x2:a)
 
 val op_cong (#a:Type) (#ops:sig) 
             (op:op{op `mem` ops}) (x:param_of op) 
-            (t1 t2:arity_of op -> template_repr a ops)
+            (t1 t2:arity_of op -> template a ops)
   : Lemma (requires (forall (y:arity_of op) . t1 y `equiv` t2 y))
           (ensures  (Node op x t1 `equiv` Node op x t2))
           [SMTPat (Node op x t1 `equiv` Node op x t2)]
